Update definition of re pos unfold (#256)
* More

* Fixes

* Compiled

* Fixes

* Correct rule

* Fix

* Fix

* Fix

* Fixing

* Fixing

* Revert

* Minor

* Fixing

* Fixing

* Fix

* Fixing

* Fixes

* Fixing

* Fix other rules

Cpc/Proofs/TermCompat.lean
@@ -151,7 +151,8 @@ abbrev str_in_re := Term.UOp UserOp.str_in_re
 abbrev seq_empty := Term.UOp1 UserOp1.seq_empty
 abbrev seq_unit := Term.UOp UserOp.seq_unit
 abbrev seq_nth := Term.UOp UserOp.seq_nth
-abbrev _at_re_unfold_pos_component := Term.UOp3 UserOp3._at_re_unfold_pos_component
+abbrev _at_re_unfold_pos_component (t r i : Term) : Term :=
+  Term.UOp3 UserOp3._at_re_unfold_pos_component t r i
 abbrev _at_strings_deq_diff (x y : Term) :=
   Term.Apply (Term.Apply (Term.UOp UserOp._at_strings_deq_diff) x) y
 abbrev _at_strings_stoi_result (x : Term) :=
